code/experimental/P256/Hacl.Impl.P256.LowLevel.fst
@@ -60,6 +60,16 @@ let lemma_t_computation2 t =
   assert_norm(18446744073709551615 + 4294967295 * pow2 64 + 18446744069414584321 * pow2 192 = prime256)
 
 
+val p256_double: arg1: felem ->  out: felem -> Stack unit 
+  (requires (fun h0 ->  live h0 arg1 /\ live h0 out /\ eq_or_disjoint arg1 out /\ as_nat h0 arg1 < prime256))
+  (ensures (fun h0 _ h1 -> modifies1 out h0 h1 /\ as_nat h1 out == (2 * as_nat h0 arg1) % prime256 /\ as_nat h1 out < prime256))
+
+let p256_double arg1 out = 
+  let t = add4 arg1 arg1 out in 
+  lemma_t_computation t;
+  reduction_prime256_2prime256_with_carry_impl t out out
+
+
 val p256_sub: arg1: felem -> arg2: felem -> out: felem -> Stack unit 
   (requires 
     (fun h0 -> live h0 out /\ live h0 arg1 /\ live h0 arg2 /\ 
@@ -77,7 +87,6 @@ val p256_sub: arg1: felem -> arg2: felem -> out: felem -> Stack unit
   ))
 
 let p256_sub arg1 arg2 out = 
-    push_frame();
     let h0 = ST.get() in 
   let t = sub4 arg1 arg2 out in 
     lemma_t_computation2 t;
@@ -102,6 +111,5 @@ let p256_sub arg1 arg2 out =
 
     substractionInDomain2Nat (felem_seq_as_nat (as_seq h0 arg1)) (felem_seq_as_nat (as_seq h0 arg2));
     inDomain_mod_is_not_mod (fromDomain_ (felem_seq_as_nat (as_seq h0 arg1)) - fromDomain_ (felem_seq_as_nat (as_seq h0 arg2)));
-    lemma_eq_funct (as_seq h2 out) (felem_sub_seq (as_seq h0 arg1) (as_seq h0 arg2));   
-    pop_frame()
+    lemma_eq_funct (as_seq h2 out) (felem_sub_seq (as_seq h0 arg1) (as_seq h0 arg2))
     
